Clean/Types/U32.lean
@@ -35,6 +35,11 @@ namespace U32
 def map {α β : Type} (x : U32 α) (f : α → β) : U32 β :=
   ⟨ f x.x0, f x.x1, f x.x2, f x.x3 ⟩
 
+lemma to_elements_map {α β : Type} (x : U32 α) (f : α → β) :
+  to_elements (map x f) = (to_elements x).map f := rfl
+
+def vals (x : U32 (F p)) : U32 ℕ := x.map ZMod.val
+
 omit [Fact (Nat.Prime p)] p_large_enough in
 /--
   Extensionality principle for U32
@@ -85,6 +90,9 @@ theorem value_xor_horner {x : U32 (F p)} (hx: x.is_normalized) : x.value =
 
 def value_nat (x: U32 ℕ) :=
   x.x0 + x.x1 * 256 + x.x2 * 256^2 + x.x3 * 256^3
+
+omit [Fact (Nat.Prime p)] p_large_enough in
+lemma vals_value (x : U32 (F p)) : x.vals.value_nat = x.value := rfl
 
 /--
   Return a 32-bit unsigned integer from a natural number, by decomposing
@@ -232,7 +240,7 @@ def circuit : FormalCircuit (F p) U32 U32 where
   main := u32_copy
   assumptions := assumptions
   spec := spec
-  local_length := 4
+  local_length _ := 4
   output inputs i0 := var_from_offset U32 i0
   soundness := by
     rintro i0 env x_var
@@ -258,10 +266,30 @@ def circuit : FormalCircuit (F p) U32 U32 where
       List.getElem_cons_zero] at h3
     simp_all
 
-end U32.Copy
+end Copy
 
 @[reducible]
-def U32.copy (x : Var U32 (F p)) : Circuit (F p) (Var U32 (F p)) :=
-  subcircuit U32.Copy.circuit x
+def copy (x : Var U32 (F p)) : Circuit (F p) (Var U32 (F p)) :=
+  subcircuit Copy.circuit x
 
-end
+namespace ByteVector
+-- results about U32 when viewed as a vector of bytes, via `to_elements` and `from_elements`
+
+omit [Fact (Nat.Prime p)] p_large_enough in
+theorem is_normalized_iff {x : U32 (F p)} :
+    x.is_normalized ↔ ∀ i (_ : i < 4), (to_elements x)[i].val < 256 := by
+  rcases x with ⟨ x0, x1, x2, x3 ⟩
+  simp only [is_normalized, to_elements, size, Vector.getElem_mk, List.getElem_toArray]
+  constructor
+  · intro h i hi
+    repeat (rcases hi with _ | hi; try simp [*, size])
+  · intro h
+    let h0 := h 0 (by decide)
+    let h1 := h 1 (by decide)
+    let h2 := h 2 (by decide)
+    let h3 := h 3 (by decide)
+    simp only [List.getElem_cons_zero, List.getElem_cons_succ] at h0 h1 h2 h3
+    simp_all
+
+end ByteVector
+end U32
